erased_swap_correct

EvmOpcodes.v
@@ -12,7 +12,6 @@ Require Import Arith.PeanoNat.
 Require Import Arith.Compare_dec.
 Require Import PeanoNat.
 
-
 Definition byte := nat.
 Definition byte32 := {items : list byte | 0 < length items /\ length items <= 32}.
 Definition word := nat.
@@ -54,7 +53,7 @@ Inductive so_instruction : Type :=
   | I_OP2 : op2 -> so_instruction
   | I_OP3 : op3 -> so_instruction
   | I_POP
-  | I_PUSH : byte32 -> so_instruction
+  | I_PUSH : word -> so_instruction (* coerced from a list of 1-32 bytes, big endian; the rest is zero *)
   | I_DUP (n : nat) : n < 16 -> so_instruction (* n is one less than DUPN *)
   | I_SWAP (n : nat) : n < 16 -> so_instruction (* n is one less than SWAPN *)
 .
@@ -63,6 +62,11 @@ Inductive mem_instruction : Type :=
   | I_MLOAD
   | I_MSTORE
   | I_MSTORE8
+.
+
+Inductive storage_instruction : Type :=
+  | I_SLOAD
+  | I_SSTORE
 .
 
 Inductive instruction : Type :=
@@ -75,6 +79,7 @@ Inductive instruction : Type :=
   | I_CALLER
   | I_CALLVALUE
   | I_CALLDATALOAD
+  | I_CALLDATASIZE
   | I_CALLDATACOPY
   | I_CODESIZE
   | I_CODECOPY
@@ -89,9 +94,8 @@ Inductive instruction : Type :=
   | I_DIFFICULTY
   | I_GASLIMIT
 
-  | I_MEM_ONLY : mem_instruction -> instruction
-  | I_SLOAD
-  | I_SSTORE
+  | I_MEMINS : mem_instruction -> instruction
+  | I_STORINS : storage_instruction -> instruction
 
   | I_JUMP
   | I_JUMPI
@@ -112,18 +116,80 @@ Inductive instruction : Type :=
 .
 
 
+Definition delta_alpha (i: instruction) : nat*nat :=
+  match i with
+    | I_STACK_ONLY I_STOP => (0, 0)
+    | I_STACK_ONLY (I_OP1 _) => (1, 1)
+    | I_STACK_ONLY (I_OP2 _) => (2, 1)
+    | I_STACK_ONLY (I_OP3 _) => (3, 1)
+    | I_STACK_ONLY I_POP => (1, 0)
+    | I_STACK_ONLY (I_PUSH _) => (0, 1)
+    | I_STACK_ONLY (I_DUP n _) => (1 + n, 2 + n)
+    | I_STACK_ONLY (I_SWAP n _) => (2 + n, 2 + n)
+    | I_SHA3 => (2, 1)
+
+    | I_ADDRESS => (0, 1)
+    | I_BALANCE => (1, 1)
+    | I_ORIGIN => (0, 1)
+    | I_CALLER => (0, 1)
+    | I_CALLVALUE => (0, 1)
+    | I_CALLDATALOAD => (1, 1)
+    | I_CALLDATASIZE => (0, 1)
+    | I_CALLDATACOPY => (3, 0)
+    | I_CODESIZE => (0, 1)
+    | I_CODECOPY => (3, 0)
+    | I_GASPRICE => (0, 1)
+    | I_EXTCODESIZE => (1, 1)
+    | I_EXTCODECOPY => (4, 0)
+
+    | I_BLOCKHASH => (1, 1)
+    | I_COINBASE => (0, 1)
+    | I_TIMESTAMP => (0, 1)
+    | I_NUMBER => (0, 1)
+    | I_DIFFICULTY => (0, 1)
+    | I_GASLIMIT => (0, 1)
+
+    | I_MEMINS I_MLOAD => (1, 1)
+    | I_MEMINS I_MSTORE => (2, 0)
+    | I_MEMINS I_MSTORE8 => (2, 0)
+    | I_STORINS I_SLOAD => (1, 1)
+    | I_STORINS I_SSTORE => (2, 0)
+
+    | I_JUMP => (1, 0)
+    | I_JUMPI => (2, 0)
+    | I_PC => (0, 1)
+
+    | I_MSIZE => (0, 1)
+    | I_GAS => (0, 1)
+    | I_JUMPDEST  => (0, 0) (* NO-OP - mark as label *)
+
+    | I_LOG n => (n + 2, 0)
+
+    | I_CREATE => (3, 1)
+    | I_CALL => (7, 1)
+    | I_CALLCODE => (7, 1)
+    | I_RETURN => (2, 0)
+    | I_DELEGATECALL => (6, 1)
+    | I_SUICIDE => (1, 10)
+  end.
+
+Definition delta (i: instruction) : nat := fst (delta_alpha i).
+Definition alpha (i: instruction) : nat := snd (delta_alpha i).
+
+Parameter SUB_BOUND : nat.
+Definition BOUND := S SUB_BOUND.
 
 (** The stack is represented as a Coq [list word]
-    plus a proof that its lenth is smaller than 1024 *)
+    plus a proof that its lenth is smaller than BOUND *)
 Record stack_t: Type := mkstack {
   stckval: list word; 
-  stcksize: length stckval < 1024
+  stcksize: length stckval < BOUND
 }.
 
-Lemma pop_lt : forall {w : word} {ws: list word}, length (w :: ws) < 1024 -> length ws < 1024.
+Lemma pop_lt : forall {w : word} {ws: list word}, length (w :: ws) < BOUND -> length ws < BOUND.
 Proof.
   intros.
-  exact (Nat.lt_lt_succ_r (length ws) 1023 (lt_S_n (length ws) 1023 H)).
+  exact (Nat.lt_lt_succ_r (length ws) SUB_BOUND (lt_S_n (length ws) SUB_BOUND H)).
 Qed.
 
 Definition eval_op1 (op : op1) (c : word) : word :=
@@ -164,10 +230,26 @@ Definition eval_op3 (op : op3) (c1 c2 c3 : word) : word :=
 Variable coerce_to_word : byte32 -> word.
 
 Definition option_mkstack (st : list word) : option stack_t :=
-  match le_lt_dec 1024 (length st) with
+  match le_lt_dec BOUND (length st) with
     | right LEN => Some (mkstack st LEN)
     | left _ => None
   end.
+
+Definition inbounds n : Prop := n < BOUND.
+Definition noflow (xs : list word) : Prop := inbounds (length xs).
+
+Definition dup (n : nat) (ws : list word) : option stack_t :=
+   match List.nth_error ws n with
+     | Some v => option_mkstack (v::ws)
+     | None => None
+   end.
+
+Definition erased_swap (n : nat) (ws : list word) : option (list word) :=
+   match skipn (1+n) ws, firstn (1+n) ws with
+     | w1 :: l1, w0 :: l0 => Some ((w1 :: l0) ++ w0 :: l1)
+     | _, _ => None
+   end.
+
 
 Lemma swap_same_length : forall {T} (w0 w1 : T) l0 l1,
   length ((w0 :: l0) ++ w1 :: l1) = length ((w1 :: l0) ++ w0 :: l1).
@@ -178,24 +260,194 @@ Proof.
   reflexivity.
 Qed.
 
-Definition inbounds n : Prop := n < 1024.
-Definition noflow (xs : list word) : Prop := inbounds (length xs).
+Lemma erased_swap_eq : forall (n : nat) (ws ws' : list word),
+  erased_swap n ws = Some ws' ->
+  length ws = length ws'.
+Proof.
+  intros n ws ws'.
+  intros.
+  unfold erased_swap in H.
+  destruct (skipn (1+n) ws) eqn:S. discriminate H.
+  destruct (firstn (1+n) ws) eqn:F. discriminate H.
+  rewrite <- (firstn_skipn (1+n) ws).
+  inversion H.
+  rewrite -> F, S.
+  rewrite -> app_comm_cons.
+  apply swap_same_length.
+Qed.
 
-Definition dup (n : nat) (ws : list word) : option stack_t :=
-   match List.nth_error ws n with
-     | Some v => option_mkstack (v::ws)
-     | None => None
-   end.
+Lemma skipn_le : forall {T} (n : nat) (ws : list T),
+  skipn n ws <> nil -> n < length ws.
+Proof.
+  induction n.
+  intros. pose (zerop (length ws)). destruct s.
+    apply length_zero_iff_nil in e. contradiction.
+    assumption.
+  intros.
+  destruct ws. simpl in H. contradiction.
+  simpl in H. apply IHn in H. simpl.
+  apply lt_n_S.
+  assumption.
+Qed.
+
+Lemma skipn_le' : forall {T} (n : nat) (ws : list T) x xs,
+  skipn n ws = x::xs -> n < length ws.
+Proof.
+  intros.
+  assert (skipn n ws <> nil).
+    intro. rewrite -> H0 in H. inversion H.
+  apply skipn_le.
+  assumption.
+Qed.
+
+Lemma skipn_res_shorter: forall {T} (n : nat) (ws : list T),
+  length (skipn n ws) <= length ws.
+Proof.
+  induction n;  auto.
+  intros. destruct ws; auto.
+  simpl.
+  apply le_S.
+  apply IHn.
+Qed.
+
+Lemma skipn_not_lengthen : forall {T} (n : nat) (ws : list T) w,
+  skipn n ws <> w::ws.
+Proof.
+  unfold not.
+  intros. assert (length (skipn n ws) <= length ws) by (apply skipn_res_shorter).
+  rewrite -> H in H0. simpl in H0.
+  apply le_S_gt in H0.
+  apply (gt_irrefl _ H0).
+Qed.
+
+Lemma skipn_short : forall {T} (xs : list T) ys,
+  skipn (length xs) (xs ++ ys) = ys.
+Proof.
+  induction xs.
+  intros. reflexivity.
+  simpl. assumption.
+Qed.
+
+Lemma cons_inj : forall {T} xs (x: T),
+  xs <> x::xs.
+Proof.
+  unfold not.
+  induction xs.
+  intros. inversion H.
+  intros. inversion H. apply IHxs in H2. assumption.
+Qed.
+
+Lemma skipn_short1 : forall {T} n  (xs : list T) y ys,
+  skipn n (xs ++ (y::ys)) = (y::ys) -> n = length xs.
+Proof.
+  induction n.
+  intros. simpl in H. rewrite <- app_nil_l in H. apply app_inv_tail in H. subst xs. reflexivity. 
+  intros.
+  destruct xs. simpl in H. apply skipn_not_lengthen in H. contradiction.
+
+  simpl in H. simpl. f_equal. apply IHn in H. assumption.
+Qed.
+
+Lemma skipn_app : forall {T} (xs : list T) y ys,
+  skipn (length xs) (xs ++ (y::ys)) = (y::ys).
+Proof.
+  induction xs.
+  intros. reflexivity.
+  intros.
+  simpl. apply IHxs.
+Qed.
+
+
+Lemma erased_swap_long : forall (n : nat) (ws ws' : list word),
+  erased_swap n ws = Some ws' ->
+  (1+n) < length ws.
+Proof.
+  intros. simpl.
+  unfold erased_swap in H.
+  destruct (skipn (1 + n) ws) eqn:Q. inversion H.
+  destruct (firstn (1 + n) ws). inversion H.
+  apply skipn_le' in Q.
+  assumption.
+Qed.
+
+Lemma erased_swap_skipn : forall w0 w1 l0 l1,
+  erased_swap (length l0) ((w0 :: l0) ++ w1 :: l1) = Some ((w1 :: l0) ++ w0 :: l1).
+Proof.
+  intros.
+  unfold erased_swap.
+  assert (1 + length l0 = length (w0::l0)) by reflexivity.
+  rewrite -> H.
+  rewrite -> firstn_app, firstn_all, minus_diag.
+  rewrite -> skipn_app, app_nil_r.
+  reflexivity.
+Qed.
+
+Lemma skipn_nil : forall {T} (n : nat) (ws : list T),
+  skipn n ws = nil -> length ws <= n.
+Proof.
+  induction n.
+  intros. simpl in H. subst ws. auto.
+  intros. simpl in H. destruct ws. apply Peano.le_0_n.
+  simpl. apply IHn in H. apply Peano.le_n_S, H.
+Qed.
+
+Lemma skipn_nil' : forall {T} (n : nat),
+  skipn n nil = (nil : list T).
+Proof.
+  destruct n; reflexivity.
+Qed.
+
+Lemma erased_swap_long' : forall (n : nat) (ws : list word),
+  1+n < length ws -> erased_swap n ws <> None.
+Proof.
+  unfold not.
+  intros.
+  unfold erased_swap in H0.
+  destruct (firstn (1 + n)) eqn:Q.
+  +  assert (1 + n <= length ws). apply lt_le_S, Nat.lt_succ_l. assumption.
+     apply firstn_length_le in H1.
+     rewrite -> Q in H1. inversion H1.
+  +
+    destruct (skipn (1 + n) ws) eqn:Q1.
+    apply skipn_nil in Q1. apply lt_not_le in H. contradiction.
+    inversion H0.
+Qed.
+
+Lemma skipn_succ : forall {T} n l (x : T) xs,
+  x :: xs = skipn n l -> xs = skipn (1 + n) l.
+Proof.
+  induction n; intros; destruct l; (try rewrite -> skipn_nil' in H; inversion H).
+  + simpl. inversion H. reflexivity.
+  + simpl in H. apply IHn in H. subst xs. destruct l; reflexivity.
+Qed.
+
+Lemma erased_swap_correct : forall (n : nat) (ws ws' : list word),
+  erased_swap n ws = Some ws'
+  -> exists w0 w1 l0 l1, ws = (w0::l0) ++ (w1::l1) /\ ws' = (w1::l0) ++ (w0::l1).
+Proof.
+  intros. unfold erased_swap in H.
+  assert ( firstn (1 + n) ws ++ skipn (1 + n) ws = ws) by apply firstn_skipn.
+  destruct ws eqn:Q. inversion H.
+  simpl in *.  destruct (skipn n l). inversion H. inversion H0.
+  exists w, w0, (firstn n l), (skipn (1+n) l).
+  assert ( firstn n l ++ skipn n l = l) by apply firstn_skipn.
+  split; [idtac | inversion H];
+    do 3 f_equal;
+    rewrite <- H1 in H2 at 2;
+    apply app_inv_head, skipn_succ in H2;
+    assumption.
+Qed.
 
 (* This is dependently-subtle... *)
-Definition swap (n : nat) (ws : list word) LEN : option stack_t :=
-   match firstn n ws, skipn n ws with
-     | w0::l0, w1::l1 => fun LEN2 => Some {|
-                            stckval := (w1 :: l0) ++ w0 :: l1;
-                            stcksize := eq_ind_r inbounds LEN2 (swap_same_length w1 w0 l0 l1)
-                         |}
+Definition swap (n : nat) (ws : list word) (LEN : noflow ws) :=
+   match firstn (1+n) ws, skipn (1+n) ws with
+     | w0 :: l0, w1 :: l1 =>
+          fun LEN2 => Some  {|
+            stckval := (w1 :: l0) ++ w0 :: l1;
+            stcksize := eq_ind_r inbounds LEN2 (swap_same_length w1 w0 l0 l1)
+          |}
      | _, _ => fun _ => None
-   end (eq_ind_r noflow LEN (firstn_skipn n ws)).
+   end (eq_ind_r noflow LEN (firstn_skipn (1+n) ws)).
 
 Definition exec_so_instr (i : so_instruction) (s : stack_t) : option stack_t :=
   match i, s with
@@ -208,7 +460,7 @@ Definition exec_so_instr (i : so_instruction) (s : stack_t) : option stack_t :=
     | I_OP3 _, _ => None
     | I_POP, mkstack (w::st) LEN => Some (mkstack st (pop_lt LEN))
     | I_POP, _ => None
-    | I_PUSH items, mkstack st _  => option_mkstack (coerce_to_word items :: st)
+    | I_PUSH item, mkstack st _  => option_mkstack (item::st)
     | I_DUP n _, mkstack ws _  => dup n ws
     | I_SWAP n _, mkstack ws LEN => swap n ws LEN
   end.
@@ -228,36 +480,100 @@ Definition exec_jump_instr (i : instruction) (pc : nat) (s : stack_t) : option n
     | _ => Some (pc + 1)
   end.
 
+Theorem exec_so_nice : forall i st st',
+  exec_so_instr i st = Some st' ->
+    let d := delta (I_STACK_ONLY i) in
+    let a := alpha (I_STACK_ONLY i) in
+    stckval st' = firstn a (stckval st') ++ skipn d (stckval st).
+Proof.
+  destruct st as [s LEN]. simpl.
+  destruct st' as [s' LEN']. simpl.
+  intros.
+  destruct (exec_so_instr i {| stckval := s; stcksize := LEN |}) eqn:Q; inversion H.
+  subst s0. clear H.
+  unfold exec_so_instr in Q.
+  destruct i.
+  + inversion Q.
+  + destruct s; inversion Q. reflexivity.
+  +
+    destruct s eqn:?. simplify_eq Q.
+    destruct l eqn:?. simplify_eq Q.
+    inversion Q.
+    reflexivity.
+  +
+    destruct s eqn:?. simplify_eq Q.
+    destruct l eqn:?. simplify_eq Q.
+    destruct l0; inversion Q.
+    reflexivity.
+  +
+    destruct s eqn:?; inversion Q.
+    reflexivity.
+  +
+    unfold option_mkstack in Q.
+    destruct (le_lt_dec BOUND (length (w :: s))); inversion Q.
+    reflexivity.
+  + (* I_DUP *)
+    unfold alpha, delta.
+    unfold dup in Q; inversion Q.
+    destruct (nth_error s n) eqn:NE; inversion Q.
+    unfold option_mkstack in Q.
+    destruct (le_lt_dec BOUND (length (w :: s))); inversion Q.
+     simpl (snd (delta_alpha (I_STACK_ONLY (I_DUP n l)))).
+     simpl (fst (delta_alpha (I_STACK_ONLY (I_DUP n l)))).
+    assert (firstn_ssn : firstn (S (S n)) (w :: s) = w :: firstn (S n) s) by reflexivity.
+    rewrite -> firstn_ssn.
+    rewrite <- app_comm_cons.
+    rewrite -> (firstn_skipn (S n) s).
+    reflexivity.
+  + (* I_SWAP *)
+    unfold alpha, delta.
+     simpl (snd (delta_alpha (I_STACK_ONLY (I_SWAP n l)))).
+     simpl (fst (delta_alpha (I_STACK_ONLY (I_SWAP n l)))).
+    rewrite <- (firstn_skipn (S (S n)) s') at 1.
+    f_equal.
+    unfold swap in Q.
 
-Require Import Vector.
+Qed.
+
 Require Import FSets.FMapWeakList.
 Module Import MapNat := FMapWeakList.Make Nat.
 Definition memory := MapNat.t word.
 
-Definition stack_read_word (bs : list word) : option word :=
-  if length bs <? 32 then None else coerce_32word_to_word (firstn 32 bs).
+Parameter mem_read_word : memory -> word -> word.
+Parameter mem_store_word : memory -> word -> word -> memory.
+Definition mem_store_byte (m: memory) (addr: word) (b: byte) : memory := add addr b m.
 
-Definition exec_mem_instr (i : mem_instruction) (m : memory) (bs : list word) : option (memory * list word) :=
-  match i with
-    | I_MLOAD => match stack_read_word bs with
-                   | Some addr => match find addr m with
-                                    | Some b => Some (m, b::bs)
-                                    | None => None
-                                  end
-                   | None => None
-                 end
-    | I_MSTORE => match stack_read_word bs with
-                   | Some addr => match find addr m with
-                                    | Some b => Some (m, b::bs)
-                                    | None => None
-                                  end
-                   | None => None
-                 end
-    | I_MSTORE8 => None
+Definition first_byte (w: word) : byte := Nat.modulo w 32.
+
+Definition exec_mem_instr (i : mem_instruction) (m : memory) (st : stack_t) : option (memory * stack_t) :=
+  match i, st with
+    | I_MLOAD, mkstack (addr::ws) LEN => Some (m, mkstack (mem_read_word m addr :: ws) LEN)
+    | I_MSTORE, mkstack (addr::val::ws) _ => Some (mem_store_word m addr val, st)
+    | I_MSTORE8, mkstack (addr::val::ws) _ => Some (mem_store_byte m addr (first_byte val), st)
+    | _, _ => None
   end.
 
 Definition storage := MapNat.t word.
+
+Definition storage_read (p: storage) (addr: word) : word :=
+  match find addr p with
+    | Some v => v
+    | None => 0
+  end.
+Definition storage_store (p: storage) (addr: word) (w: word) : memory :=
+  add addr w p.
+
+(* storage should be indexed by contract id *)
+Definition exec_storage_instr (i : storage_instruction) (p : storage) (st : stack_t) : option (storage * stack_t) :=
+  match i, st with
+    | I_SLOAD, mkstack (addr::ws) LEN => Some (p, mkstack (storage_read p addr :: ws) LEN)
+    | I_SSTORE, mkstack (addr::val::ws) _ => Some (storage_store p addr val, st)
+    | _, _ => None
+  end.
+
 Variable size : nat.
+
+Require Import Vector.
 Variable code : Vector.t instruction size.
 
 
